Simple proofs added.

Reforge.fst
@@ -7,6 +7,7 @@ open FStar.String
 open Statements
 open GlobalState
 open CommonFunctions
+open FStar.List
 
 (*  function that mints `amount` of tokens to `account` *)
 let _mint   (state: global_state)
@@ -69,6 +70,16 @@ let _mint   (state: global_state)
                                     *)
                                     let _ = assert (FStar.UInt256.eq (FStar.UInt256.add _accountBalance amount) _accountBalance_upd) in
 
+                                    (*
+                                       Update state with the new event - emit Transfer(address(0), account, amount);                                                            
+                                    *)
+                                    let events_length_old = length (!s).events_ in 
+                                    s := {!s with events_ = Transfer Solidity.default_address account amount :: (!s).events_};
+
+                                    // verify that the events_ list has grown - event has been emitted
+                                    let events_length_new = length (!s).events_ in 
+                                    let _ = assert(events_length_old < events_length_new) in 
+
                 // return updated state
                 (Some(), !s))
                     | _ -> (raise Solidity.SolidityOverflow)
@@ -96,6 +107,9 @@ let reforge     (state: global_state)
             if not (check_requirement_1 && check_requirement_2) then 
                 raise Solidity.SolidityInsufficientRole
             else ();
+
+            // Verify that account must have either of the two roles (BRIDGE_OWNER_ROLE or MINTER_ROLE)
+            let _ = assert(check_requirement_1 || check_requirement_2) in 
             
             // ii)   check if requirement is satisfied (transaction has not been initialized yet)
             let check_requirement_3 = Solidity.get (!s)._transactions transaction in 
@@ -103,6 +117,9 @@ let reforge     (state: global_state)
                 // if it is `true` then we need to raise an exception
                 raise Solidity.SolidityTransactionAlreadyProcessed
             else ();
+
+            // verify that each transaciton can be issued only once
+            let _ = assert(not check_requirement_3) in 
 
             // iii) mint `amount` of tokens to account `to`
             let (ret__, st__) = _mint (!s) to amount in 
@@ -115,6 +132,10 @@ let reforge     (state: global_state)
                                     let check_fee_not_zero = FStar.UInt256.gt fee (Solidity.to_uint 0) in 
                                     if check_fee_not_zero then
                                         (
+
+                                        // Verify that fee is always greater than 0 (semi-definite number)
+                                        let _ = assert(FStar.UInt256.gt fee (Solidity.to_uint 0)) in
+
                                         // iv) mint `fee` to `_bridgeOwner`
                                         let (ret__2, st__2) = _mint (!s) (!s)._bridgeOwner fee in 
                                             match ret__2 with 
@@ -126,8 +147,14 @@ let reforge     (state: global_state)
                                                             s := {!s with _transactions = Solidity.set 
                                                                                           (!s)._transactions transaction true };
 
+                                                            let events_length_old = length (!s).events_ in 
+
                                                             // vi)  update state with the new event - emit Reforged(to, amount, transaction);
                                                             s := {!s with events_ = Reforged to amount transaction :: (!s).events_};
+
+                                                            // verify that the events_ list has grown - event has been emitted
+                                                            let events_length_new = length (!s).events_ in 
+                                                            let _ = assert(events_length_old < events_length_new) in 
 
                                                             // return updated state
                                                             (Some (), !s))
@@ -139,8 +166,14 @@ let reforge     (state: global_state)
                                         // v)  set transaciton to true
                                         s := {!s with _transactions = Solidity.set (!s)._transactions transaction true };
 
+                                        let events_length_old = length (!s).events_ in 
+
                                         // vi)  update state with the new event - emit Reforged(to, amount, transaction);
                                         s := {!s with events_ = Reforged to amount transaction :: (!s).events_};
+
+                                        // verify that the events_ list has grown - event has been emitted
+                                        let events_length_new = length (!s).events_ in 
+                                        let _ = assert(events_length_old < events_length_new) in 
 
                                         // return updated state
                                         (Some (), !s)
